* it actually compiles!!!

Common.v
@@ -1,12 +1,8 @@
-Require Import FunctionalExtensionality.
-Require Import Nat.
 Require Export List.
 Require Export Coq.Lists.ListSet.
 Require Export Sorting.Permutation.
 Require Export Setoid.
-Local Open Scope nat_scope.
-
-Require Import Basic.
+Require Export Basic.
 
 Section Labels.
 
@@ -28,221 +24,68 @@ end.
 
 End Labels.
 
-Section Expressions.
+Module Type DecType.
 
-Definition Value := nat.
+Parameter t : Type.
+Parameter eq_dec : forall x y:t, {x = y} + {x <> y}.
 
-Lemma eq_value_dec : forall (e e' : Value), { e = e' } + { e <> e' }.
+End DecType.
+
+Module DecidableType (Import M:DecType).
+
+Definition eqb (x y:t) := if (eq_dec x y) then true else false.
+
+Notation "x '=?' y" := (eqb x y).
+
+Lemma eqb_eq : forall x y, (x =? y) = true <-> x = y.
 Proof.
-decide equality.
+intros; unfold eqb; elim (eq_dec x y); intros; split; auto.
+intro; discriminate H.
 Qed.
 
-
-Inductive Expr : Type :=
- | this : Expr
- | zero : Expr
- | succ_this : Expr
-.
-
-Lemma eq_expr_dec : forall (e e' : Expr), { e = e' } + { e <> e' }.
+Lemma eqb_neq : forall x y, (x =? y) = false <-> x <> y.
 Proof.
-decide equality.
+intros; split; intro.
++ contradict H. rewrite <- eqb_eq in H. rewrite H. discriminate.
++ case_eq (x =? y); auto. intro. rewrite eqb_eq in H0. elim H; auto.
 Qed.
 
-Definition eqb_expr (e:Expr) (e':Expr) : bool :=
-match e, e' with
- | this, this => true
- | zero, zero => true
- | succ_this, succ_this => true
- | _, _ => false
-end.
-
-End Expressions.
-
-Section Pids.
-
-Definition Pid := nat.
-
-Definition eq_pid := Nat.eq.
-
-Definition eqb_pid := Nat.eqb.
-
-Lemma eq_pid_dec : forall (p p':Pid), { p = p' } + { p <> p' }.
+Lemma eqb_refl : forall x, (x =? x) = true.
 Proof.
-decide equality.
+intro. rewrite eqb_eq. auto.
 Qed.
 
+Lemma eqb_sym : forall x y, (x =? y) = (y =? x).
+Proof.
+intros. case_eq (x =? y); intro; symmetry.
++ rewrite eqb_eq. symmetry. rewrite <- eqb_eq. auto.
++ rewrite eqb_neq. rewrite eqb_neq in H. auto.
+Qed.
+
+End DecidableType.
+
+Module Type Eval (Expression Value : DecType).
+
+Parameter eval : Expression.t -> Value.t -> Value.t.
+
+End Eval.
+
+(*
 Definition set_add_pid := set_add eq_pid_dec.
-Definition set_union_pid := set_union eq_pid_dec.
 Definition set_inter_pid := set_inter eq_pid_dec.
 
 Definition eq_pidset (s:set Pid) (s':set Pid) : Prop := Permutation s s'.
-
-(*
-Lemma set_add_pid_char :
-  forall (p:Pid) (P:set Pid),
-  ~(In p P) -> (set_add_pid p P) = P ++ p::nil.
-Proof.
-intros.
-induction P.
-easy.
-simpl in H.
-apply deMorganNotOr in H.
-inversion H.
-set (myH := IHP H1).
-simpl.
-rewrite myH.
-induction eq_pid_dec.
-symmetry in a0.
-contradiction.
-trivial.
-Qed.
-
-Lemma not_in_rev_pid : forall (p:Pid) (P:set Pid), ~(In p P) -> ~(In p (rev P)).
-Proof.
-intros.
-red.
-red in H.
-induction P.
-trivial.
-simpl.
-simpl in H.
-apply or_over_impl in H.
-inversion_clear H.
-set (H3 := (IHP H1)).
-intros.
-apply in_app_iff in H.
-inversion H.
-apply (H3 H2).
-inversion H2.
-apply (H0 H4).
-inversion H4.
-Qed.
-
-Lemma set_union_pid_nil :
-  forall (P:set Pid), (NoDup P) ->
-  (set_union eq_pid_dec nil P) = (rev P).
-Proof.
-intros.
-induction P.
-trivial.
-simpl.
-inversion H.
-rewrite IHP.
-apply set_add_pid_char.
-set (myH := (in_rev P a)).
-inversion myH.
-apply (not_in_rev_pid a P H2).
-trivial.
-Qed.
-
-Lemma pidseteq_perm :
-  forall (p q:Pid) (P:set Pid),
-  eq_pidset (p :: P ++ q :: nil) (q :: p :: P).
-Proof.
-intros.
-red.
-induction P.
-simpl (p :: nil ++ q :: nil).
-apply perm_swap.
-simpl (p :: (a :: P) ++ q :: nil).
-apply Permutation_sym.
-rewrite perm_swap.
-apply perm_skip.
-rewrite perm_swap.
-apply perm_skip.
-apply Permutation_cons_append.
-Qed.
-
-Lemma set_union_pid_el :
-  forall (p:Pid) (P:set Pid),
-  ~(In p P) -> (eq_pidset (set_add_pid p P) (p::P)).
-Proof.
-intros.
-induction P.
-easy.
-simpl.
-simpl in H.
-apply deMorganNotOr in H.
-inversion H.
-destruct eq_pid_dec.
-rewrite e in H0.
-contradiction.
-set (myH := IHP H1).
-rewrite set_add_pid_char.
-rewrite set_add_pid_char in myH.
-apply pidseteq_perm.
-trivial.
-trivial.
-Qed.
-
-Lemma nodup_pid_app :
-  forall (P Q:set Pid),
-  (NoDup (P ++ Q)) -> (NoDup P) /\ (NoDup Q).
-Proof.
-intros.
-induction P.
-split.
-apply NoDup_nil.
-trivial.
-split.
-simpl in H.
-apply NoDup_cons_iff in H.
-inversion_clear H.
-apply NoDup_cons.
-(* ~ In a (P ++ Q) -> ~ In a P *)
-set (myH := (in_or_app P Q a)).
-apply or_over_impl in myH; inversion_clear myH.
-intro.
-apply H0.
-apply in_or_app.
-auto.
-elim IHP; auto.
-simpl in H.
-inversion H.
-elim IHP; auto.
-Qed.
-
-Lemma set_union_pid_char : forall (P Q:set Pid),
-  (NoDup (P ++ Q)) ->
-  (set_union_pid P Q) = P ++ rev Q.
-Proof.
-intros.
-elim (nodup_pid_app _ _ H); intros.
-induction Q.
-simpl.
-symmetry; apply app_nil_r.
-simpl.
-inversion_clear H1; rewrite IHQ; auto.
-rewrite set_add_pid_char; auto.
-rewrite app_assoc; auto.
-apply NoDup_remove_2.
-apply (Permutation_NoDup Pid (P ++ a :: Q) (P ++ a :: rev Q)); auto.
-apply Permutation_app_head.
-apply Permutation_cons; auto.
-apply Permutation_rev.
-apply NoDup_remove_1 with a; auto.
-Qed.
-
-Lemma set_union_pid_sets : forall (P Q:set Pid),
-  (NoDup (P ++ Q)) ->
-  (eq_pidset (set_union_pid P Q) (set_union_pid Q P)).
-Proof.
-intros.
-repeat rewrite set_union_pid_char; auto.
-apply Permutation_trans with (rev P ++ Q).
-apply Permutation_app.
-apply Permutation_rev.
-symmetry; apply Permutation_rev.
-apply Permutation_app_comm.
-apply Permutation_NoDup with (P ++ Q); auto.
-apply Permutation_app_comm.
-Qed.
 *)
 
-End Pids.
+Module State (P V : DecType).
 
-Section State.
+Module Pdec := DecidableType P.
+Module Vdec := DecidableType V.
+
+Definition Pid := P.t.
+Definition Pid_dec := Pdec.eqb.
+Definition Value := V.t.
+Definition Value_dec := Vdec.eqb.
 
 Definition State := Pid -> Value.
 
@@ -326,11 +169,10 @@ induction P.
 (* P is empty *)
 + left. red. intros. contradiction.
 (* a :: P *)
-+ assert (SHP := eq_value_dec (s1 a) (s2 a)).
-  case IHP, SHP.
-  - left. apply eq_state_cons; assumption.
-  - right. contradict n. apply eq_state_hd with P, n.
-  - right. contradict n. apply eq_state_tl with a, n.
++ case IHP.
+  - case_eq (Value_dec (s1 a) (s2 a)).
+    * left. apply eq_state_cons; auto. apply (Vdec.eqb_eq); auto.
+    * right. contradict H. rewrite not_false_iff_true. rewrite Vdec.eqb_eq. apply eq_state_hd with P, H.
   - right. contradict n. apply eq_state_tl with a, n.
 Qed.
 
@@ -361,36 +203,59 @@ Add Parametric Relation P : State (eq_state P)
   reflexivity proved by (eq_state_refl P)
   symmetry proved by (eq_state_sym P)
   transitivity proved by (eq_state_trans P)
-  as eq_setate_rel.
+  as eq_state_rel.
 
 (* TODO: Perhaps Add Parametric Morphism *)
 
-(** Expression evaluation given a value for the place-holder this *)
-Definition evaluate_on_value (e:Expr) (v:Value) : Value :=
-match e with
- | zero => 0
- | this => v
- | succ_this => S v
-end.
-
-(** Expression evaluation on the state of a process *)
-Definition evaluate_on_state (e:Expr) (s:State) (p:Pid) : Value := evaluate_on_value e (s p).
-
 Definition update (s:State) (p:Pid) (v:Value) : State :=
-  fun (q:Pid) => if (p =? q) then v else (s q).
+  fun (q:Pid) => if (Pid_dec p q) then v else (s q).
 
-Lemma update_read : forall (s:State) (p:Pid) (v:Value),
-  update s p v p = v.
+Lemma update_read : forall (s:State) (p:Pid) (v:Value), update s p v p = v.
 Proof.
   intros.
   unfold update.
-  rewrite <- beq_nat_refl; auto.
+  rewrite Pdec.eqb_refl; auto.
 Qed.
 
-Lemma read_update : forall s p q v e, p<>q -> evaluate_on_state e (update s q v) p = evaluate_on_state e s p.
+Lemma update_read' : forall (s:State) (p q:Pid) (v:Value), p <> q -> update s p v q = s q.
+Proof.
+  intros.
+  unfold update, Pid_dec.
+  rewrite <- Pdec.eqb_neq in H; rewrite H; auto.
+Qed.
+
+Lemma update_update : forall (s:State) (p:Pid) (v1 v2:Value) (P : list Pid),
+  eq_state P (update (update s p v2) p v1) (update s p v1).
+Proof.
 intros.
-assert (q<>p); auto.
-induction e; simpl; unfold update; auto; rewrite <- Nat.eqb_neq in H0; rewrite H0; auto.
+red.
+unfold update.
+unfold update.
+intro q.
+case_eq (Pid_dec p q); trivial.
+Qed.
+
+Definition eq_state_ext (s1 s2: State) : Prop := forall p, s1 p = s2 p.
+
+Lemma update_update_ext : forall (s:State) (p:Pid) (v1 v2:Value),
+  eq_state_ext (update (update s p v2) p v1) (update s p v1).
+Proof.
+intros.
+red.
+unfold update.
+unfold update.
+intro q.
+case_eq (Pid_dec p q); trivial.
+Qed.
+
+Lemma update_independent : forall s p q e e', p<>q ->
+  eq_state_ext (update (update s q e') p e) (update (update s p e) q e').
+Proof.
+red; intros.
+unfold update.
+case_eq (Pid_dec p p0); case_eq (Pid_dec q p0); auto; intros.
+elim H; rewrite Pdec.eqb_eq in H0; rewrite Pdec.eqb_eq in H1.
+transitivity p0; auto.
 Qed.
 
 Lemma update_not_in : forall (s:State) (p:Pid) (v:Value) (P:list Pid),
@@ -404,54 +269,10 @@ induction P.
   destruct H.
   split.
   - unfold update. 
-    case_eq (p =? a); auto. 
-    intro H1. apply beq_nat_true in H1. 
+    case_eq (Pid_dec p a); auto. 
+    intro H1. rewrite Pdec.eqb_eq in H1. 
     elim H. contradiction. 
   - apply IHP, H0.
-Qed.
-
-Lemma update_update : forall (s:State) (p:Pid) (v1 v2:Value) (P : list Pid),
-  eq_state P (update (update s p v2) p v1) (update s p v1).
-Proof.
-intros.
-red.
-unfold update.
-unfold update.
-intro q.
-case_eq (p =? q); trivial.
-Qed.
-
-(* Lemma updrate_swap :  forall (s: State) *)
-
-Fixpoint list_to_state (l : list (Pid * Value)) : State :=
-match l with
-| nil => fun _ => 0
-| (p,v)::l' => update (list_to_state l') p v
-end.
-
-(* Eval compute in (list_to_state ((0,0)::(1,2)::(0,1)::nil)). *)
-
-Definition eq_state_ext (s1 s2: State) : Prop := forall p, s1 p = s2 p.
-
-Lemma update_update_ext : forall (s:State) (p:Pid) (v1 v2:Value),
-  eq_state_ext (update (update s p v2) p v1) (update s p v1).
-Proof.
-intros.
-red.
-unfold update.
-unfold update.
-intro q.
-case_eq (p =? q); trivial.
-Qed.
-
-Lemma update_independent : forall s p q e e', p<>q ->
-  eq_state_ext (update (update s q e') p e) (update (update s p e) q e').
-Proof.
-red; intros.
-unfold update.
-case_eq (p =? p0); case_eq (q =? p0); auto; intros.
-elim H; rewrite Nat.eqb_eq in H0; rewrite Nat.eqb_eq in H1.
-transitivity p0; auto.
 Qed.
 
 End State.
