MC_old.v
@@ -1,22 +1,10 @@
 Require Export Basic.
 Require Export Common.
 
+(* Can we get rid of this? *)
+Require Export Coq.Program.Equality.
+
 Local Open Scope nat_scope.
-
-Module MCBase (P E V: DecType) (Import Ev : Eval E V).
-
-Module Import St := State P V.
-Module Pdec := DecidableType P.
-Module Edec := DecidableType E.
-Module Vdec := DecidableType V.
-
-Definition Pid := P.t.
-Definition Pid_dec := Pdec.eqb.
-Definition Expr := E.t.
-Definition Expr_dec := Edec.eqb.
-Definition Value := V.t.
-Definition Value_dec := Vdec.eqb.
-Definition State := St.State.
 
 Section Syntax.
 
@@ -26,11 +14,9 @@ Inductive Eta : Type :=
  | Sel : Pid -> Pid -> Label -> Eta
 .
 
-Lemma eta_eq_dec : forall (eta eta':Eta), { eta = eta' } + { eta <> eta' }.
+Lemma eq_eta_dec : forall (eta eta':Eta), { eta = eta' } + { eta <> eta' }.
 Proof.
-decide equality; try apply P.eq_dec.
-+ apply E.eq_dec.
-+ decide equality.
+repeat decide equality.
 Qed.
 
 Definition disjoint (p q r s:Pid) :=  p <> r /\ p <> s /\ q <> r /\ q <> s.
@@ -66,10 +52,9 @@ Inductive Choreography : Type :=
  | Cond : Pid -> Pid -> Choreography -> Choreography -> Choreography
 .
 
-Lemma chor_eq_dec : forall (C C':Choreography), { C = C' } + { C <> C' }.
+Lemma eq_chor_dec : forall (C C':Choreography), { C = C' } + { C <> C' }.
 Proof.
-decide equality; try apply P.eq_dec.
-apply eta_eq_dec.
+repeat decide equality.
 Qed.
 
 (** A choreography is well-formed if it does not contain self-communications. *)
@@ -89,8 +74,6 @@ match e with
 end
 .
 
-Definition set_union_pid := set_union P.eq_dec.
-
 Fixpoint pn (C:Choreography) : list Pid :=
 match C with
 | End => nil
@@ -102,33 +85,33 @@ end
 Lemma pn_is_set (C:Choreography) : WellFormed C -> NoDup(pn C).
 Proof.
 induction C; intros.
-+ (* End *)
-  apply NoDup_nil.
-+ (* e; C *)
-  simpl.
-  apply set_union_nodup.
-  simpl in H.
-  induction e; inversion_clear H.
-  - (* Com *)
-    simpl; repeat apply NoDup_cons; simpl; auto.
-    intro.
-    inversion_clear H; auto.
-    apply NoDup_nil.
-  - (* Sel *)
-    simpl; repeat apply NoDup_cons; simpl; auto.
-    intro.
-    inversion_clear H; auto.
-    apply NoDup_nil.
-   - induction e; inversion H; auto.
-+ (* Cond *)
-  inversion H.
-  inversion_clear H1.
-  simpl.
-  repeat apply set_union_nodup; auto.
-  simpl; repeat apply NoDup_cons; simpl; auto.
-  intro.
-  inversion_clear H1; auto.
-  apply NoDup_nil.
+(* End *)
+apply NoDup_nil.
+(* e; C *)
+simpl.
+apply set_union_nodup.
+simpl in H.
+induction e; inversion_clear H.
+(* Com *)
+simpl; repeat apply NoDup_cons; simpl; auto.
+intro.
+inversion_clear H; auto.
+apply NoDup_nil.
+(* Sel *)
+simpl; repeat apply NoDup_cons; simpl; auto.
+intro.
+inversion_clear H; auto.
+apply NoDup_nil.
+induction e; inversion H; auto.
+(* Cond *)
+inversion H.
+inversion_clear H1.
+simpl.
+repeat apply set_union_nodup; auto.
+simpl; repeat apply NoDup_cons; simpl; auto.
+intro.
+inversion_clear H1; auto.
+apply NoDup_nil.
 Qed.
 
 End Syntax.
@@ -199,12 +182,20 @@ Lemma Precongr_step_to : forall C C', Precongr_step C C' -> Precongr C C'.
 intros; apply Trans with C'; auto; apply Refl.
 Qed.
 
+Example sanity_check : Precongr ( Com 0 this 1; If 2 == 3 Then (Com 4 succ_this 3; End) Else (Com 3 zero 2; End) )
+                                ( If 2 == 3 Then (Com 0 this 1; Com 4 succ_this 3; End) Else (Com 3 zero 2; Com 0 this 1; End) ).
+Proof.
+ eapply Trans.
+ apply EtaCond; split; auto.
+ apply CtxCond'.
+ apply Refl.
+ apply Precongr_step_to; apply EtaEta.
+ split; auto.
+Qed.
+
 Definition Configuration : Type := Choreography * State.
 
 Definition WellFormedConf (conf:Configuration) : Prop := WellFormed( fst conf ).
-
-(** Expression evaluation on the state of a process *)
-Definition evaluate_on_state (e:Expr) (s:State) (p:Pid) : Value := eval e (s p).
 
 (** One-step and multi-step reduction. Multi-step reduction is simply a reflexive and transitive closure. *)
 Inductive MCTo : Configuration -> Configuration -> Prop :=
@@ -246,13 +237,22 @@ Notation "c --->* c'" := (MCToStar c c') (at level 50, left associativity).
 Notation "C1 ~<= C2" := (Precongr C1 C2) (at level 50, left associativity).
 Notation "C1 ~< C2" := (Precongr_step C1 C2) (at level 50, left associativity).
 
+(* Notation "C1 \u22e0 C2" := (not (C1 \u227c C2)) (at level 50). *)
+
 Section Semantics_Props.
 
-Lemma read_update : forall s p q v e, p<>q -> evaluate_on_state e (update s q v) p = evaluate_on_state e s p.
+(** * Induction principles for one-step reduction in MC. *)
+Lemma MCTo_induction : forall (P:Choreography -> State -> Choreography -> State -> Prop),
+  (forall p e q C s, P (p#e --> q; C) s C (update s q (evaluate_on_state e s p))) ->
+  (forall p q l C s, P (Sel p q l; C) s C s) ->
+  (forall p q C1 C2 s, s p = s q -> P (If p == q Then C1 Else C2) s C1 s) ->
+  (forall p q C1 C2 s, s p <> s q -> P (If p == q Then C1 Else C2) s C2 s) ->
+  (forall C1 C1' C2 C2' s1 s2, Precongr C1 C1' -> Precongr C2' C2 -> P C1' s1 C2' s2 -> P C1 s1 C2 s2) ->
+  forall C s C' s', (C,s) ---> (C',s') -> P C s C' s'.
 Proof.
 intros.
-unfold evaluate_on_state.
-rewrite update_read'; auto.
+dependent induction H4; auto.
+apply H3 with C1' C2'; auto.
 Qed.
 
 (** * Properties of precongruence. *)
@@ -280,7 +280,7 @@ Qed.
 Lemma not_End_precongr' : forall C:Choreography, C ~<= End -> C = End.
 Proof.
 intros.
-elim (chor_eq_dec C End); auto.
+elim (eq_chor_dec C End); auto.
 intro.
 elim not_End_precongr with C End; auto.
 Qed.
@@ -338,6 +338,86 @@ induction H0; auto.
 apply IHPrecongr; apply not_terminated_precongr' with C1; auto.
 Qed.
 
+Lemma terminated_does_not_reduce : forall C C' s s', terminated C -> ~(C,s) ---> (C',s').
+Proof.
+intros; intro.
+rewrite (not_End_precongr' _ H) in H0; clear H.
+dependent induction H0.
+assert (C1' = End).
++ clear H1 IHMCTo C2' C' H0 s s'.
+  dependent induction H; auto.
+  apply IHPrecongr; inversion H.
++ rewrite H2 in IHMCTo, H1; clear H C1' H2.
+  apply IHMCTo with C2' s s'; auto.
+Qed.
+
+Lemma not_terminated_weird : forall {C s C' s' C''}, (C,s) ---> (C',s') -> C ~<= C'' -> ~terminated C''.
+Proof.
+intros; intro.
+red in H1; simpl in H1; rewrite (not_End_precongr' _ H1) in H0.
+rewrite (not_End_precongr' _ H0) in H.
+revert H; apply terminated_does_not_reduce; apply Refl.
+Qed.
+
+(** The size of a choreography, as the minimal number of reductions until we reach a terminal. *)
+Fixpoint size (C:Choreography) : nat :=
+  match C with
+  | End => 0
+  | eta; C' => 1 + size C'
+  | If p == q Then C1 Else C2 => 1 + min (size C1) (size C2)
+  end.
+
+Lemma precongr_size_ge : forall C C', C ~<= C' -> size C <= size C'.
+intros.
+induction H; simpl; auto with arith.
++ transitivity (size C2); auto.
+  clear IHPrecongr H0; induction H; simpl; auto with arith.
+  - set (s1 := size C1); set (s2 := size C2); set (s0 := size C0); set (s4 := size C4).
+    repeat apply le_n_S.
+    rewrite Nat.min_assoc.
+    rewrite <- (Nat.min_assoc s1 s2 s0).
+    rewrite (Nat.min_comm s2 s0).
+    repeat rewrite Nat.min_assoc; auto.
+  - apply le_n_S.
+    apply Nat.min_glb.
+    * transitivity (size C'); auto; apply Nat.le_min_l.
+    * apply Nat.le_min_r.
+  - apply le_n_S.
+    apply Nat.min_glb.
+    * apply Nat.le_min_l.
+    * transitivity (size C'); auto; apply Nat.le_min_r.
+Qed.
+
+(** Some useful characterizations using size. *)
+Lemma size_0_End : forall C, size C = 0 -> C = End.
+Proof.
+induction C; simpl; auto; intros; inversion H.
+Qed.
+
+Lemma MCTo_End_size : forall C s s', (C,s) ---> (End, s') -> size C = 1.
+Proof.
+intros.
+assert (size C <> 0).
+* intro.
+  rewrite (size_0_End _ H0) in H.
+  apply (terminated_does_not_reduce _ _ _ _ (Refl _) H).
+* generalize (eq_refl End).
+  generalize H0.
+  apply MCTo_induction with (P:=fun C _ C' _ => size C <> 0 -> C' = End -> size C = 1) (s:=s) (C':=End) (s':=s'); simpl; auto; intros.
+  + rewrite H2; auto.
+  + rewrite H2; auto.
+  + rewrite H3; auto.
+  + rewrite H3; rewrite Nat.min_comm; auto.
+  + rewrite H5 in H2; clear H5.
+    generalize (not_End_precongr' _ H2); clear H2; intro.
+    generalize (precongr_size_ge _ _ H1); intro.
+    rewrite H3 in H5; auto.
+    - inversion H5; auto.
+      elim H4; auto with arith.
+    - intro; apply H4.
+      rewrite H6 in H5; auto with arith.
+Qed.
+
 (** Head reductions (do not use structural precongruence). *)
 
 Definition HeadTo (c:Configuration) : ~ (terminated (fst c)) -> Configuration.
@@ -346,7 +426,7 @@ elim H; apply terminated_iff_End; auto.
 destruct e.
 apply (c, update s p0 (evaluate_on_state e s p)).
 apply (c, s).
-apply (if (Value_dec (s p) (s p0)) then (c1, s) else (c2, s)).
+apply (if ((s p) =? (s p0)) then (c1, s) else (c2, s)).
 Defined.
 
 Lemma HeadTo_wd : forall c H H', HeadTo c H = HeadTo c H'.
@@ -382,9 +462,11 @@ induction e.
 apply C_Com.
 apply C_Sel.
 simpl.
-case_eq (Value_dec (s p) (s p0)); intros.
-+ apply C_Then; apply Vdec.eqb_eq; auto.
-+ apply C_Else; apply Vdec.eqb_neq; auto.
+case_eq (Nat.eqb (s p) (s p0)); intros.
+apply C_Then.
+apply beq_nat_true; auto.
+apply C_Else.
+apply beq_nat_false; auto.
 Qed.
 
 (*
@@ -467,7 +549,7 @@ induction C; intro s.
   set (c1 := HeadTo c0 NTc0).
   assert (c1 = (HeadTo c0 NTc0)); auto.
   induction c1 as (C1, s1).
-  case_eq (Value_dec (s p) (s p0)); intro G.
+  case_eq (Nat.eqb (s p) (s p0)); intro G.
   + elim (IHC1 s1); intros c' Hc'.
     inversion_clear c'; exists c'; split; auto.
     inversion_clear Hc'. 
@@ -498,206 +580,6 @@ End Semantics_Props.
 
 Notation "c $ H -H-> c'" := (HeadTo c H = c') (at level 50).
 
-Section Weighted_Relations.
-
-Inductive Precongr_weighted : nat -> Choreography -> Choreography -> Prop :=
-  | PBase : forall {C}, Precongr_weighted 0 C C
-  | PStep : forall {n C} C' {C''}, C ~< C' -> Precongr_weighted n C' C'' -> Precongr_weighted (S n) C C''
-.
-
-Lemma Precongr_to_weighted : forall C C', C ~<= C' -> exists n, Precongr_weighted n C C'.
-Proof.
-intros; induction H.
-+ exists 0; apply PBase.
-+ elim IHPrecongr; intros n Hn.
-  exists (S n); apply PStep with C2; auto.
-Qed.
-
-Lemma Precongr_weighted_to : forall n C C', Precongr_weighted n C C' -> C ~<= C'.
-Proof.
-induction n; intros; inversion H.
-+ apply Refl.
-+ apply Trans with C'0; auto.
-Qed.
-
-Inductive MCTo_weighted : nat -> Configuration -> Configuration  -> Prop :=
-  | Base : forall {c c'} H, c$H -H-> c' -> MCTo_weighted 0 c c'
-  | Cons : forall {n k m C1} C1' C2' {C2 s1 s2}, Precongr_weighted n C1 C1' -> MCTo_weighted k (C1',s1) (C2',s2) -> Precongr_weighted m C2' C2 -> MCTo_weighted (S (n+k+m)) (C1,s1) (C2,s2)
-.
-
-Lemma MCTo_weighted_to : forall n c c', MCTo_weighted n c c' -> c ---> c'.
-Proof.
-assert (forall n k, k < n -> forall c c', MCTo_weighted k c c' -> c ---> c').
-2: intro; apply H with (S n); auto.
-induction n; intros.
-+ inversion H.
-+ inversion H0.
-  - rewrite <- H2; apply HeadTo_Soundness.
-  - apply C_Struct with C1' C2'.
-    * apply Precongr_weighted_to with n0; auto.
-    * apply Precongr_weighted_to with m; auto.
-    * apply IHn with k0; auto.
-      rewrite <- H4 in H; red in H.
-      apply lt_le_trans with (S (n0+k0+m)); auto with arith.
-Qed.
-
-Lemma MCTo_to_weighted : forall c c', c ---> c' -> exists n, MCTo_weighted n c c'.
-Proof.
-intros; induction H.
-+ exists 0; set (H := eta_not_terminated (p#e-->q) C); apply Base with H; auto.
-+ exists 0; set (H := eta_not_terminated (Sel p q l) C); apply Base with H; auto.
-+ exists 0; set (H0 := cond_not_terminated p q C1 C2); apply Base with H0.
-  simpl; rewrite <- Vdec.eqb_eq in H.
-  unfold Value_dec; rewrite H; auto.
-+ exists 0; set (H0 := cond_not_terminated p q C1 C2); apply Base with H0.
-  simpl; rewrite <- Vdec.eqb_neq in H.
-  unfold Value_dec; rewrite H; auto.
-+ elim IHMCTo; clear IHMCTo; intros k Hk.
-  elim (Precongr_to_weighted _ _ H); intros n Hn.
-  elim (Precongr_to_weighted _ _ H0); intros m Hm.
-  exists (S (n+k+m)).
-  apply Cons with C1' C2'; auto.
-Qed.
-
-End Weighted_Relations.
-
-Notation "C $ n '~<n' C'" := (Precongr_weighted n C C') (at level 50).
-Notation "c $ n -n-> c'" := (MCTo_weighted n c c') (at level 50).
-
-Section Applications.
-
-(** Some results that require stronger induction principles, which we obtain through weight. *)
-
-Lemma terminated_does_not_reduce : forall C C' s s', terminated C -> ~(C,s) ---> (C',s').
-Proof.
-intros; intro.
-rewrite (not_End_precongr' _ H) in H0; clear H.
-elim (MCTo_to_weighted _ _ H0); clear H0; intros n Hn.
-assert (forall k, k <= n -> ~(End,s)$k -n-> (C',s')); intros.
-2: apply H with n; auto.
-clear C Hn; revert k H s C' s'.
-induction n; intros; intro; inversion H0; try (apply H1; apply Refl).
-+ rewrite <- H4 in H; inversion H.
-+ clear C1 H1 s1 H2 C2 H3 s2 H5.
-  generalize (Precongr_weighted_to _ _ _ H6); clear H6; intro.
-  generalize (End_precongr _ H1); clear H1; intro.
-  rewrite H1 in H7.
-  eapply (IHn k0).
-  2: apply H7.
-  rewrite <- H4 in H; apply le_S_n in H.
-  transitivity (n0+k0+m); auto with arith.
-Qed.
-
-Lemma not_terminated_weird : forall {C s C' s' C''}, (C,s) ---> (C',s') -> C ~<= C'' -> ~terminated C''.
-Proof.
-intros; intro.
-red in H1; simpl in H1; rewrite (not_End_precongr' _ H1) in H0.
-rewrite (not_End_precongr' _ H0) in H.
-revert H; apply terminated_does_not_reduce; apply Refl.
-Qed.
-
-(** Useful induction principle. *)
-Lemma MCTo_induction : forall (P:Choreography -> State -> Choreography -> State -> Prop),
-  (forall p e q C s, P (p#e --> q; C) s C (update s q (evaluate_on_state e s p))) ->
-  (forall p q l C s, P (Sel p q l; C) s C s) ->
-  (forall p q C1 C2 s, s p = s q -> P (If p == q Then C1 Else C2) s C1 s) ->
-  (forall p q C1 C2 s, s p <> s q -> P (If p == q Then C1 Else C2) s C2 s) ->
-  (forall C1 C1' C2 C2' s1 s2, Precongr C1 C1' -> Precongr C2' C2 -> P C1' s1 C2' s2 -> P C1 s1 C2 s2) ->
-  forall C s C' s', (C,s) ---> (C',s') -> P C s C' s'.
-Proof.
-intros.
-elim (MCTo_to_weighted _ _ H4); intros n Hn; clear H4.
-assert (forall k, k <= n -> (C,s)$k -n-> (C',s') -> P C s C' s'); intros.
-2: apply H4 with n; auto.
-clear Hn; revert k H4 C s C' s' H5; induction n; intros.
-+ rewrite <- (le_n_0_eq _ H4) in H5; inversion H5.
-  induction C.
-  - contradiction H6; red; simpl; apply Refl.
-  - induction e; inversion H7; auto.
-  - inversion H7; revert H11.
-    case_eq (Value_dec (s p) (s p0)); intros Hs Hc'; inversion Hc'; rewrite <- H12.
-    * rewrite Vdec.eqb_eq in Hs; auto.
-    * rewrite Vdec.eqb_neq in Hs; auto.
-+ inversion H5.
-  induction C.
-  - contradiction H6; red; simpl; apply Refl.
-  - induction e; inversion H7; auto.
-  - inversion H7; revert H12.
-    case_eq (Value_dec (s p) (s p0)); intros Hs Hc'; inversion Hc'; rewrite <- H13.
-    * rewrite Vdec.eqb_eq in Hs; auto.
-    * rewrite Vdec.eqb_neq in Hs; auto.
- - apply H3 with C1' C2'; auto.
-    * apply Precongr_weighted_to with n0; auto.
-    * apply Precongr_weighted_to with m; auto.
-    * apply IHn with k0; auto.
-      rewrite <- H9 in H4.
-      apply le_S_n in H4.
-      transitivity (n0+k0+m); auto with arith.
-Qed.
-
-(** The size of a choreography, as the minimal number of reductions until we reach a terminal. *)
-Fixpoint size (C:Choreography) : nat :=
-  match C with
-  | End => 0
-  | eta; C' => 1 + size C'
-  | If p == q Then C1 Else C2 => 1 + min (size C1) (size C2)
-  end.
-
-Lemma precongr_size_ge : forall C C', C ~<= C' -> size C <= size C'.
-intros.
-induction H; simpl; auto with arith.
-+ transitivity (size C2); auto.
-  clear IHPrecongr H0; induction H; simpl; auto with arith.
-  - set (s1 := size C1); set (s2 := size C2); set (s0 := size C0); set (s4 := size C4).
-    repeat apply le_n_S.
-    rewrite Nat.min_assoc.
-    rewrite <- (Nat.min_assoc s1 s2 s0).
-    rewrite (Nat.min_comm s2 s0).
-    repeat rewrite Nat.min_assoc; auto.
-  - apply le_n_S.
-    apply Nat.min_glb.
-    * transitivity (size C'); auto; apply Nat.le_min_l.
-    * apply Nat.le_min_r.
-  - apply le_n_S.
-    apply Nat.min_glb.
-    * apply Nat.le_min_l.
-    * transitivity (size C'); auto; apply Nat.le_min_r.
-Qed.
-
-(** Some useful characterizations using size. *)
-Lemma size_0_End : forall C, size C = 0 -> C = End.
-Proof.
-induction C; simpl; auto; intros; inversion H.
-Qed.
-
-Lemma MCTo_End_size : forall C s s', (C,s) ---> (End, s') -> size C = 1.
-Proof.
-intros.
-assert (size C <> 0).
-* intro.
-  rewrite (size_0_End _ H0) in H.
-  apply (terminated_does_not_reduce _ _ _ _ (Refl _) H).
-* generalize (eq_refl End).
-  generalize H0.
-  apply MCTo_induction with (P:=fun C _ C' _ => size C <> 0 -> C' = End -> size C = 1) (s:=s) (C':=End) (s':=s'); simpl; auto; intros.
-  + rewrite H2; auto.
-  + rewrite H2; auto.
-  + rewrite H3; auto.
-  + rewrite H3; rewrite Nat.min_comm; auto.
-  + rewrite H5 in H2; clear H5.
-    generalize (not_End_precongr' _ H2); clear H2; intro.
-    generalize (precongr_size_ge _ _ H1); intro.
-    rewrite H3 in H5; auto.
-    - inversion H5; auto.
-      elim H4; auto with arith.
-    - intro; apply H4.
-      rewrite H6 in H5; auto with arith.
-Qed.
-
-End Applications.
-
-Require Import Coq.Program.Equality.
-
 Section Representation_principles.
 
 (** Head reductions propagate by precongruence. *)
@@ -714,7 +596,7 @@ dependent induction H1; intros.
     apply CtxEta; apply EtaEta; auto.
   - exists (Sel p p0 l; eta2; eta1; C); split; auto.
     apply CtxEta; apply EtaEta; auto.
-  - case_eq (Value_dec (s p) (s p0)); intro; rewrite H2 in H3; inversion H3.
+  - case_eq (s p =? s p0); intro; rewrite H2 in H3; inversion H3.
     * exists (If p == p0 Then eta2; eta1; C Else C0_2); split.
       apply CtxThen; apply EtaEta; auto.
       intro; simpl; rewrite <- H6; rewrite H2; auto.
@@ -728,7 +610,7 @@ dependent induction H1; intros.
     apply CtxEta; apply EtaCond; auto.
   - exists (Sel p0 p1 l; If p == q Then eta; C1 Else (eta; C2)); split; auto.
     apply CtxEta; apply EtaCond; auto.
-  - case_eq (Value_dec (s p0) (s p1)); intro; rewrite H3 in H4; inversion H4.
+  - case_eq (s p0 =? s p1); intro; rewrite H3 in H4; inversion H4.
     * exists (If p0 == p1 Then If p == q Then eta; C1 Else (eta; C2) Else C4); split.
       apply CtxThen; apply EtaCond; auto.
       intro; simpl; rewrite <- H7; rewrite H3; auto.
@@ -742,7 +624,7 @@ dependent induction H1; intros.
     apply CtxEta; apply CondEta; auto.
   - exists (Sel p0 p1 l; eta; If p == q Then C1 Else C2); split; auto.
     apply CtxEta; apply CondEta; auto.
-  - case_eq (Value_dec (s p0) (s p1)); intro; rewrite H3 in H4; inversion H4.
+  - case_eq (s p0 =? s p1); intro; rewrite H3 in H4; inversion H4.
     * exists (If p0 == p1 Then eta; If p == q Then C1 Else C2 Else C4); split.
       apply CtxThen; apply CondEta; auto.
       intro; simpl; rewrite <- H7; rewrite H3; auto.
@@ -756,7 +638,7 @@ dependent induction H1; intros.
     apply CtxEta; apply CondCond; auto.
   - exists (Sel p0 p1 l;(If r == s0 Then If p == q Then C1 Else C3 Else (If p == q Then C2 Else C4))); split; auto.
     apply CtxEta; apply CondCond; auto.
-  - case_eq (Value_dec (s p0) (s p1)); intro; rewrite H2 in H3; inversion H3.
+  - case_eq (s p0 =? s p1); intro; rewrite H2 in H3; inversion H3.
     * exists (If p0 == p1 Then (If r == s0 Then If p == q Then C1 Else C3 Else (If p == q Then C2 Else C4)) Else C6); split; auto.
       apply CtxThen; apply CondCond; auto.
       intro; simpl; rewrite <- H6; rewrite H2; auto.
@@ -770,7 +652,7 @@ dependent induction H1; intros.
     apply CtxEta; apply CtxEta; auto.
   - exists (Sel p p0 l; eta; C2); split; auto.
     apply CtxEta; apply CtxEta; auto.
-  - case_eq (Value_dec (s p) (s p0)); intro; rewrite H2 in H3; inversion H3.
+  - case_eq (s p =? s p0); intro; rewrite H2 in H3; inversion H3.
     * exists (If p == p0 Then eta; C2 Else C4); split; auto.
       apply CtxThen; apply CtxEta; auto.
       intro; simpl; rewrite <- H6; rewrite H2; auto.
@@ -784,7 +666,7 @@ dependent induction H1; intros.
     apply CtxEta; apply CtxThen; auto.
   - exists (Sel p0 p1 l; If p == q Then C'' Else C); split; auto.
     apply CtxEta; apply CtxThen; auto.
-  - case_eq (Value_dec (s p0) (s p1)); intro; rewrite H2 in H3; inversion H3.
+  - case_eq (s p0 =? s p1); intro; rewrite H2 in H3; inversion H3.
     * exists (If p0 == p1 Then If p == q Then C'' Else C Else C0_2); split; auto.
       apply CtxThen; apply CtxThen; auto.
       intro; simpl; rewrite <- H6; rewrite H2; auto.
@@ -798,7 +680,7 @@ dependent induction H1; intros.
     apply CtxEta; apply CtxElse; auto.
   - exists (Sel p0 p1 l; If p == q Then C Else C''); split; auto.
     apply CtxEta; apply CtxElse; auto.
-  - case_eq (Value_dec (s p0) (s p1)); intro; rewrite H2 in H3; inversion H3.
+  - case_eq (s p0 =? s p1); intro; rewrite H2 in H3; inversion H3.
     * exists (If p0 == p1 Then If p == q Then C Else C'' Else C0_2); split; auto.
       apply CtxThen; apply CtxElse; auto.
       intro; simpl; rewrite <- H6; rewrite H2; auto.
@@ -852,42 +734,46 @@ revert C' s' H0; induction H1; intros.
     * apply Precongr_step_to; apply CondEta; auto.
     * apply Refl.
     * apply C_Sel.
-+ exists C'; split; auto; inversion H2; revert H4; case_eq (Value_dec (s p) (s q)); intros.
++ exists C'; split; auto; inversion H2; revert H4; case_eq (s p =? s q); intros.
   - eapply C_Struct.
     * apply Precongr_step_to; apply EtaCond; auto.
     * apply Refl.
-    * apply C_Then; apply Vdec.eqb_eq; auto.
+    * apply C_Then; apply Nat.eqb_eq; auto.
   - eapply C_Struct.
     * apply Precongr_step_to; apply EtaCond; auto.
     * apply Refl.
-    * apply C_Else; apply Vdec.eqb_neq; auto.
-+ exists C'; split; auto; inversion H1; revert H3; case_eq (Value_dec (s p) (s q)); intros.
+    * apply C_Else; rewrite <- Nat.eqb_eq; intro.
+      rewrite H3 in H5; inversion H5.
++ exists C'; split; auto; inversion H1; revert H3; case_eq (s p =? s q); intros.
   - eapply C_Struct.
     * apply Precongr_step_to; apply CondCond; apply disjoint_sym; auto.
     * apply Refl.
-    * apply C_Then; apply Vdec.eqb_eq; auto.
+    * apply C_Then; apply Nat.eqb_eq; auto.
   - eapply C_Struct.
     * apply Precongr_step_to; apply CondCond; apply disjoint_sym; auto.
     * apply Refl.
-    * apply C_Else; apply Vdec.eqb_neq; auto.
+    * apply C_Else; rewrite <- Nat.eqb_eq; intro.
+      rewrite H2 in H4; inversion H4.
 + exists C2; inversion H0; induction eta; inversion H3; split; auto.
   - apply C_Com.
   - rewrite <- H4; auto.
   - apply C_Sel.
   - rewrite <- H4; auto.
-+ inversion H0; revert H3; case_eq (Value_dec (s p) (s q)); intros; inversion H3.
++ inversion H0; revert H3; case_eq (s p =? s q); intros; inversion H3.
   - exists C''; split.
-    * apply C_Then; apply Vdec.eqb_eq; rewrite <- H6; auto.
+    * apply C_Then; apply Nat.eqb_eq; rewrite <- H6; auto.
     * rewrite <- H5; auto.
   - exists C; split.
-    * rewrite <- H5; apply C_Else; rewrite <- Vdec.eqb_neq; rewrite <- H6; auto.
+    * rewrite <- H5; apply C_Else; rewrite <- Nat.eqb_eq; intro.
+      rewrite H6 in H2; rewrite H4 in H2; inversion H2.
     * rewrite H5; auto.
-+ inversion H0; revert H3; case_eq (Value_dec (s p) (s q)); intros; inversion H3.
++ inversion H0; revert H3; case_eq (s p =? s q); intros; inversion H3.
   - exists C; split.
-    * rewrite <- H5; apply C_Then; apply Vdec.eqb_eq; rewrite <- H6; auto.
+    * rewrite <- H5; apply C_Then; apply Nat.eqb_eq; rewrite <- H6; auto.
     * rewrite H5; auto.
   - exists C''; split.
-    * apply C_Else; apply Vdec.eqb_neq; rewrite <- H6; auto.
+    * apply C_Else; rewrite <- Nat.eqb_eq; intro.
+      rewrite H6 in H2; rewrite H4 in H2; inversion H2.
     * rewrite <- H5; auto.
 Qed.
 
@@ -921,100 +807,108 @@ induction H1.
     exists C; eexists; eexists; split; [apply C_Sel | split; [apply C_Sel | intro]].
     rewrite <- H5, H7; auto.
 + right.
-  induction eta; inversion H0; revert H2; simpl; case_eq (Value_dec (s p) (s q)); intros; inversion H4.
+  induction eta; inversion H0; revert H2; simpl; case_eq (s p =? s q); intros; inversion H4.
   - (* Then/Com *)
     exists C1, s', s'.
     split; [idtac | split; [idtac | intro; reflexivity]].
     * rewrite <- H9, <- H6; apply C_Then; auto.
       inversion_clear H1; inversion_clear H3.
-      repeat rewrite update_read'; auto.
-      apply Vdec.eqb_eq; auto.
+      rewrite H6.
+      change (evaluate_on_state this s' p = evaluate_on_state this s' q).
+      rewrite <- H6; repeat rewrite read_update with (e:=this); auto.
+      rewrite Nat.eqb_eq in H2; auto.
     * rewrite <- H9, <- H6; apply C_Com.
   - (* Else/Com *)
     exists C2, s', s'.
     split; [idtac | split; [idtac | intro; reflexivity]].
     * rewrite <- H9; rewrite <- H6; apply C_Else; auto.
       inversion_clear H1; inversion_clear H3.
-      repeat rewrite update_read'; auto.
-      apply Vdec.eqb_neq; auto.
+      rewrite H6.
+      change (evaluate_on_state this s' p <> evaluate_on_state this s' q).
+      rewrite <- H6; repeat rewrite read_update with (e:=this); auto.
+      rewrite Nat.eqb_neq in H2; auto.
     * rewrite <- H9, <- H6; apply C_Com.
   - (* Then/Sel *)
     exists C1, s', s'.
     split; [idtac | split; [idtac | intro; reflexivity]].
     * apply C_Then; auto.
       inversion_clear H1; inversion_clear H3.
-      rewrite <- H6; apply Vdec.eqb_eq; auto.
+      rewrite <- H6; rewrite Nat.eqb_eq in H2; auto.
     * rewrite <- H9, <- H6; apply C_Sel.
   - (* Else/Sel *)
     exists C2, s', s'.
     split; [idtac | split; [idtac | intro; reflexivity]].
     * rewrite <- H6; apply C_Else; auto.
       inversion_clear H1; inversion_clear H3.
-      apply Vdec.eqb_neq; auto.
+      rewrite Nat.eqb_neq in H2; auto.
     * rewrite <- H9, <- H6; apply C_Sel.
 + right.
-  induction eta; inversion H2; revert H0; simpl; case_eq (Value_dec (s p) (s q)); intros; inversion H4.
+  induction eta; inversion H2; revert H0; simpl; case_eq (s p =? s q); intros; inversion H4.
   - (* Com/Then *)
     exists C1, s''', s'''.
     split; [idtac | split; [idtac | intro; reflexivity]].
     * rewrite <- H9, <- H6; apply C_Com.
     * rewrite <- H9; rewrite <- H6; apply C_Then; auto.
       inversion_clear H1; inversion_clear H3.
-      repeat rewrite update_read'; auto.
-      apply Vdec.eqb_eq; auto.
+      rewrite H6.
+      change (evaluate_on_state this s''' p = evaluate_on_state this s''' q).
+      rewrite <- H6; repeat rewrite read_update with (e:=this); auto.
+      rewrite Nat.eqb_eq in H0; auto.
   - (* Com/Else *)
     exists C2, s''', s'''.
     split; [idtac | split; [idtac | intro; reflexivity]].
     * rewrite <- H9, <- H6; apply C_Com.
     * rewrite <- H9; rewrite <- H6; apply C_Else; auto.
       inversion_clear H1; inversion_clear H3.
-      repeat rewrite update_read'; auto.
-      apply Vdec.eqb_neq; auto.
+      rewrite H6.
+      change (evaluate_on_state this s''' p <> evaluate_on_state this s''' q).
+      rewrite <- H6; repeat rewrite read_update with (e:=this); auto.
+      rewrite Nat.eqb_neq in H0; auto.
   - (* Sel/Then *)
     exists C1, s''', s'''.
     split; [idtac | split; [idtac | intro; reflexivity]].
     * rewrite <- H9, <- H6; apply C_Sel.
     * apply C_Then; auto.
       inversion_clear H1; inversion_clear H3.
-      rewrite <- H6; apply Vdec.eqb_eq; auto.
+      rewrite <- H6; rewrite Nat.eqb_eq in H0; auto.
   - (* Sel/Else *)
     exists C2, s''', s'''.
     split; [idtac | split; [idtac | intro; reflexivity]].
     * rewrite <- H9, <- H6; apply C_Sel.
     * rewrite <- H6; apply C_Else; auto.
       inversion_clear H1; inversion_clear H3.
-      apply Vdec.eqb_neq; auto.
+      rewrite Nat.eqb_neq in H0; auto.
 + right.
   revert H0 H2; rename H1 into H'; destroy H'.
-  simpl; case_eq (Value_dec (s p) (s q)); simpl; case_eq (Value_dec (s r) (s s0)); intros;
+  simpl; case_eq (s p =? s q); simpl; case_eq (s r =? s s0); intros;
   inversion H5; clear H5; inversion H6; clear H6.
   - (* Then/Then *)
     rewrite <- H10, <- H9; exists C1, s, s; split;
     [apply C_Then | split; [apply C_Then | intro; auto]];
-    rewrite Vdec.eqb_eq in H3, H4; auto.
+    rewrite Nat.eqb_eq in H3, H4; auto.
   - (* Else/Then *)
     rewrite <- H10, <- H9; exists C2, s, s; split;
     [apply C_Else | split; [apply C_Then | intro; auto]];
-    rewrite Vdec.eqb_neq in H3; rewrite Vdec.eqb_eq in H4; auto.
+    rewrite Nat.eqb_neq in H3; rewrite Nat.eqb_eq in H4; auto.
   - (* Then/Else *)
     rewrite <- H10, <- H9; exists C3, s, s; split;
     [apply C_Then | split; [apply C_Else | intro; auto]];
-    rewrite Vdec.eqb_eq in H3; rewrite Vdec.eqb_neq in H4; auto.
+    rewrite Nat.eqb_eq in H3; rewrite Nat.eqb_neq in H4; auto.
   - (* Else/Else *)
     rewrite <- H10, <- H9; exists C4, s, s; split;
     [apply C_Else | split; [apply C_Else | intro; auto]];
-    rewrite Vdec.eqb_neq in H3, H4; auto.
+    rewrite Nat.eqb_neq in H3, H4; auto.
 + (* Com *)
   left; clear IHPrecongr_step.
   induction eta; inversion H0; inversion H2; split; try rewrite <- H4, <- H6; auto.
   transitivity s; auto.
 + left; clear IHPrecongr_step.
   inversion H0; inversion H2; revert H4 H5.
-  case_eq (Value_dec (s p) (s q)); intros; inversion H4; inversion H5; split; try (transitivity s; auto);
+  case_eq (s p =? s q); intros; inversion H4; inversion H5; split; try (transitivity s; auto);
   rewrite <- H7, <- H9; auto.
 + left; clear IHPrecongr_step.
   inversion H0; inversion H2; revert H4 H5.
-  case_eq (Value_dec (s p) (s q)); intros; inversion H4; inversion H5; split; try (transitivity s; auto);
+  case_eq (s p =? s q); intros; inversion H4; inversion H5; split; try (transitivity s; auto);
   rewrite <- H7; rewrite <- H9; auto.
 Qed.
 
@@ -1026,10 +920,10 @@ dependent induction H.
 + exists (p#e-->q;C'); exists C'; repeat split; auto; apply Refl.
 + exists (Sel p q l; C'); exists C'; repeat split; auto; apply Refl.
 + exists (If p == q Then C' Else C2); exists C'; repeat split; try apply Refl.
-  intros; simpl; rewrite <- Vdec.eqb_eq in H; unfold Value_dec; rewrite H; auto.
+  intros; simpl; rewrite <- Nat.eqb_eq in H; rewrite H; auto.
 + exists (If p == q Then C1 Else C'); exists C'; repeat split; try apply Refl.
-  intros; simpl; rewrite <- Vdec.eqb_eq in H.
-  unfold Value_dec; rewrite (not_true_is_false _ H); auto.
+  intros; simpl; rewrite <- Nat.eqb_eq in H.
+  rewrite (not_true_is_false _ H); auto.
 + elim (IHMCTo _ _ _ _ (JMeq_refl _) (JMeq_refl _)); clear IHMCTo; intros.
   rename x into C''; inversion_clear H2.
   rename x into C'''; inversion_clear H3.
@@ -1054,6 +948,5 @@ exists C3; split; auto.
 apply Precongr_Trans with C1; auto.
 Qed.
 
-End Representation_principles.
 
-End MCBase.
+End Representation_principles.
