Common_old.v
@@ -1,0 +1,457 @@
+Require Import FunctionalExtensionality.
+Require Import Nat.
+Require Export List.
+Require Export Coq.Lists.ListSet.
+Require Export Sorting.Permutation.
+Require Export Setoid.
+Local Open Scope nat_scope.
+
+Require Import Basic.
+
+Section Labels.
+
+Inductive Label : Type :=
+ | left : Label
+ | right : Label
+.
+Lemma eq_label_dec : forall (l l' : Label), { l = l' } + { l <> l' }.
+Proof.
+decide equality.
+Qed.
+
+Definition eqb_label (l l':Label) : bool :=
+match l, l' with
+ | left, left => true
+ | right, right => true
+ | _, _ => false
+end.
+
+End Labels.
+
+Section Expressions.
+
+Definition Value := nat.
+
+Lemma eq_value_dec : forall (e e' : Value), { e = e' } + { e <> e' }.
+Proof.
+decide equality.
+Qed.
+
+
+Inductive Expr : Type :=
+ | this : Expr
+ | zero : Expr
+ | succ_this : Expr
+.
+
+Lemma eq_expr_dec : forall (e e' : Expr), { e = e' } + { e <> e' }.
+Proof.
+decide equality.
+Qed.
+
+Definition eqb_expr (e:Expr) (e':Expr) : bool :=
+match e, e' with
+ | this, this => true
+ | zero, zero => true
+ | succ_this, succ_this => true
+ | _, _ => false
+end.
+
+End Expressions.
+
+Section Pids.
+
+Definition Pid := nat.
+
+Definition eq_pid := Nat.eq.
+
+Definition eqb_pid := Nat.eqb.
+
+Lemma eq_pid_dec : forall (p p':Pid), { p = p' } + { p <> p' }.
+Proof.
+decide equality.
+Qed.
+
+Definition set_add_pid := set_add eq_pid_dec.
+Definition set_union_pid := set_union eq_pid_dec.
+Definition set_inter_pid := set_inter eq_pid_dec.
+
+Definition eq_pidset (s:set Pid) (s':set Pid) : Prop := Permutation s s'.
+
+(*
+Lemma set_add_pid_char :
+  forall (p:Pid) (P:set Pid),
+  ~(In p P) -> (set_add_pid p P) = P ++ p::nil.
+Proof.
+intros.
+induction P.
+easy.
+simpl in H.
+apply deMorganNotOr in H.
+inversion H.
+set (myH := IHP H1).
+simpl.
+rewrite myH.
+induction eq_pid_dec.
+symmetry in a0.
+contradiction.
+trivial.
+Qed.
+
+Lemma not_in_rev_pid : forall (p:Pid) (P:set Pid), ~(In p P) -> ~(In p (rev P)).
+Proof.
+intros.
+red.
+red in H.
+induction P.
+trivial.
+simpl.
+simpl in H.
+apply or_over_impl in H.
+inversion_clear H.
+set (H3 := (IHP H1)).
+intros.
+apply in_app_iff in H.
+inversion H.
+apply (H3 H2).
+inversion H2.
+apply (H0 H4).
+inversion H4.
+Qed.
+
+Lemma set_union_pid_nil :
+  forall (P:set Pid), (NoDup P) ->
+  (set_union eq_pid_dec nil P) = (rev P).
+Proof.
+intros.
+induction P.
+trivial.
+simpl.
+inversion H.
+rewrite IHP.
+apply set_add_pid_char.
+set (myH := (in_rev P a)).
+inversion myH.
+apply (not_in_rev_pid a P H2).
+trivial.
+Qed.
+
+Lemma pidseteq_perm :
+  forall (p q:Pid) (P:set Pid),
+  eq_pidset (p :: P ++ q :: nil) (q :: p :: P).
+Proof.
+intros.
+red.
+induction P.
+simpl (p :: nil ++ q :: nil).
+apply perm_swap.
+simpl (p :: (a :: P) ++ q :: nil).
+apply Permutation_sym.
+rewrite perm_swap.
+apply perm_skip.
+rewrite perm_swap.
+apply perm_skip.
+apply Permutation_cons_append.
+Qed.
+
+Lemma set_union_pid_el :
+  forall (p:Pid) (P:set Pid),
+  ~(In p P) -> (eq_pidset (set_add_pid p P) (p::P)).
+Proof.
+intros.
+induction P.
+easy.
+simpl.
+simpl in H.
+apply deMorganNotOr in H.
+inversion H.
+destruct eq_pid_dec.
+rewrite e in H0.
+contradiction.
+set (myH := IHP H1).
+rewrite set_add_pid_char.
+rewrite set_add_pid_char in myH.
+apply pidseteq_perm.
+trivial.
+trivial.
+Qed.
+
+Lemma nodup_pid_app :
+  forall (P Q:set Pid),
+  (NoDup (P ++ Q)) -> (NoDup P) /\ (NoDup Q).
+Proof.
+intros.
+induction P.
+split.
+apply NoDup_nil.
+trivial.
+split.
+simpl in H.
+apply NoDup_cons_iff in H.
+inversion_clear H.
+apply NoDup_cons.
+(* ~ In a (P ++ Q) -> ~ In a P *)
+set (myH := (in_or_app P Q a)).
+apply or_over_impl in myH; inversion_clear myH.
+intro.
+apply H0.
+apply in_or_app.
+auto.
+elim IHP; auto.
+simpl in H.
+inversion H.
+elim IHP; auto.
+Qed.
+
+Lemma set_union_pid_char : forall (P Q:set Pid),
+  (NoDup (P ++ Q)) ->
+  (set_union_pid P Q) = P ++ rev Q.
+Proof.
+intros.
+elim (nodup_pid_app _ _ H); intros.
+induction Q.
+simpl.
+symmetry; apply app_nil_r.
+simpl.
+inversion_clear H1; rewrite IHQ; auto.
+rewrite set_add_pid_char; auto.
+rewrite app_assoc; auto.
+apply NoDup_remove_2.
+apply (Permutation_NoDup Pid (P ++ a :: Q) (P ++ a :: rev Q)); auto.
+apply Permutation_app_head.
+apply Permutation_cons; auto.
+apply Permutation_rev.
+apply NoDup_remove_1 with a; auto.
+Qed.
+
+Lemma set_union_pid_sets : forall (P Q:set Pid),
+  (NoDup (P ++ Q)) ->
+  (eq_pidset (set_union_pid P Q) (set_union_pid Q P)).
+Proof.
+intros.
+repeat rewrite set_union_pid_char; auto.
+apply Permutation_trans with (rev P ++ Q).
+apply Permutation_app.
+apply Permutation_rev.
+symmetry; apply Permutation_rev.
+apply Permutation_app_comm.
+apply Permutation_NoDup with (P ++ Q); auto.
+apply Permutation_app_comm.
+Qed.
+*)
+
+End Pids.
+
+Section State.
+
+Definition State := Pid -> Value.
+
+(** Equivalence of states up to a set of processes *)
+Definition eq_state (P : list Pid) (s1: State) (s2: State) : Prop := 
+  forall p, In p P -> s1 p = s2 p.
+
+(*
+Definition eq_state (P : set Pid) (s1: State) (s2: State) : Prop :=
+set_fold_right (fun p => fun b => b /\ (s1 p = s2 p)) P True.
+*)
+
+Lemma eq_state_neq : forall p P s1 s2, 
+  s1 p <> s2 p -> In p P -> ~ eq_state P s1 s2.
+Proof.
+intros. red. intros.
+red in H1.
+apply H1 in H0.
+contradiction.
+Qed.
+
+Lemma eq_state_nil : forall s1 s2, eq_state nil s1 s2.
+Proof.
+intros. red. intros. contradiction.
+Qed.
+
+Lemma eq_state_cons : forall p P s1 s2, 
+  s1 p = s2 p -> eq_state P s1 s2 -> eq_state (p::P) s1 s2.
+Proof.
+intros. red. intros.
+inversion H1.
+(* head *)
++ rewrite <- H2. assumption.
+(* tail *)
++ apply H0, H2.
+Qed.
+
+Lemma eq_state_hd : forall p P s1 s2, 
+  eq_state (p::P) s1 s2 -> s1 p = s2 p.
+Proof.
+intros. apply H, in_eq.
+Qed.
+
+Lemma eq_state_tl : forall p P s1 s2, 
+  eq_state (p::P) s1 s2 -> eq_state P s1 s2.
+Proof.
+intros. red. intros. apply H, in_cons, H0.
+Qed.
+
+Lemma eq_state_cons_iff : forall p P s1 s2, 
+  eq_state (p::P) s1 s2 <-> s1 p = s2 p /\ eq_state P s1 s2.
+Proof.
+split.
++ split; [apply eq_state_hd with P|apply eq_state_tl with p]; apply H.
++ intros. destruct H. apply eq_state_cons; auto.
+Qed.
+
+Lemma eq_state_app : forall P1 P2 s1 s2,
+  eq_state P1 s1 s2 -> eq_state P2 s1 s2 -> eq_state (P1 ++ P2) s1 s2.
+Proof.
+intros. red. intros.
+apply in_app_or in H1.
+destruct H1.
+(* p in P1 *)
++ apply H, H1.
+(* p in P2 *)
++ apply H0, H1.
+Qed.
+
+Lemma eq_state_split : forall P1 P2 s1 s2,
+  eq_state (P1 ++ P2) s1 s2 -> eq_state P1 s1 s2 /\ eq_state P2 s1 s2.
+Proof.
+intros. split; red; intros; apply H, in_or_app; auto.
+Qed.
+
+Lemma eq_state_dec : forall P s1 s2, 
+  { eq_state P s1 s2 } + { ~eq_state P s1 s2}. 
+Proof.
+intros.
+induction P.
+(* P is empty *)
++ left. red. intros. contradiction.
+(* a :: P *)
++ assert (SHP := eq_value_dec (s1 a) (s2 a)).
+  case IHP, SHP.
+  - left. apply eq_state_cons; assumption.
+  - right. contradict n. apply eq_state_hd with P, n.
+  - right. contradict n. apply eq_state_tl with a, n.
+  - right. contradict n. apply eq_state_tl with a, n.
+Qed.
+
+Lemma eq_state_refl : forall P, reflexive _ (eq_state P).
+Proof.
+repeat (red; intros). auto.
+Qed.
+
+Lemma eq_state_sym : forall P, symmetric _ (eq_state P).
+Proof.
+repeat (red; intros).
+apply symmetry, H, H0.
+Qed.
+
+Lemma eq_state_trans : forall P, transitive _ (eq_state P).
+Proof.
+red.
+intros.
+red.
+red in H, H0.
+intros.
+specialize (H p H1).
+specialize (H0 p H1).
+rewrite H. apply H0.
+Qed.
+
+Add Parametric Relation P : State (eq_state P)
+  reflexivity proved by (eq_state_refl P)
+  symmetry proved by (eq_state_sym P)
+  transitivity proved by (eq_state_trans P)
+  as eq_setate_rel.
+
+(* TODO: Perhaps Add Parametric Morphism *)
+
+(** Expression evaluation given a value for the place-holder this *)
+Definition evaluate_on_value (e:Expr) (v:Value) : Value :=
+match e with
+ | zero => 0
+ | this => v
+ | succ_this => S v
+end.
+
+(** Expression evaluation on the state of a process *)
+Definition evaluate_on_state (e:Expr) (s:State) (p:Pid) : Value := evaluate_on_value e (s p).
+
+Definition update (s:State) (p:Pid) (v:Value) : State :=
+  fun (q:Pid) => if (p =? q) then v else (s q).
+
+Lemma update_read : forall (s:State) (p:Pid) (v:Value),
+  update s p v p = v.
+Proof.
+  intros.
+  unfold update.
+  rewrite <- beq_nat_refl; auto.
+Qed.
+
+Lemma read_update : forall s p q v e, p<>q -> evaluate_on_state e (update s q v) p = evaluate_on_state e s p.
+intros.
+assert (q<>p); auto.
+induction e; simpl; unfold update; auto; rewrite <- Nat.eqb_neq in H0; rewrite H0; auto.
+Qed.
+
+Lemma update_not_in : forall (s:State) (p:Pid) (v:Value) (P:list Pid),
+  ~In p P -> eq_state P s (update s p v).
+Proof.
+intros.
+induction P.
++ apply eq_state_nil.
++ apply eq_state_cons_iff. 
+  apply not_in_cons in H.
+  destruct H.
+  split.
+  - unfold update. 
+    case_eq (p =? a); auto. 
+    intro H1. apply beq_nat_true in H1. 
+    elim H. contradiction. 
+  - apply IHP, H0.
+Qed.
+
+Lemma update_update : forall (s:State) (p:Pid) (v1 v2:Value) (P : list Pid),
+  eq_state P (update (update s p v2) p v1) (update s p v1).
+Proof.
+intros.
+red.
+unfold update.
+unfold update.
+intro q.
+case_eq (p =? q); trivial.
+Qed.
+
+(* Lemma updrate_swap :  forall (s: State) *)
+
+Fixpoint list_to_state (l : list (Pid * Value)) : State :=
+match l with
+| nil => fun _ => 0
+| (p,v)::l' => update (list_to_state l') p v
+end.
+
+(* Eval compute in (list_to_state ((0,0)::(1,2)::(0,1)::nil)). *)
+
+Definition eq_state_ext (s1 s2: State) : Prop := forall p, s1 p = s2 p.
+
+Lemma update_update_ext : forall (s:State) (p:Pid) (v1 v2:Value),
+  eq_state_ext (update (update s p v2) p v1) (update s p v1).
+Proof.
+intros.
+red.
+unfold update.
+unfold update.
+intro q.
+case_eq (p =? q); trivial.
+Qed.
+
+Lemma update_independent : forall s p q e e', p<>q ->
+  eq_state_ext (update (update s q e') p e) (update (update s p e) q e').
+Proof.
+red; intros.
+unfold update.
+case_eq (p =? p0); case_eq (q =? p0); auto; intros.
+elim H; rewrite Nat.eqb_eq in H0; rewrite Nat.eqb_eq in H1.
+transitivity p0; auto.
+Qed.
+
+End State.
